

The derivative of $f(x) = g(x) \cdot h(x)$, with $g(x) = x^2$ and $h(x) = \sin(x)$ equals

$$f'(x)$$

The derivative of $f(x) = g(x) \cdot h(x)$, with $g(x) = x^2$ and $h(x) = \sin(x)$ equals

$$f'(x) = g'(x) \cdot h(x) +$$

The derivative of $f(x) = g(x) \cdot h(x)$, with $g(x) = x^2$ and $h(x) = \sin(x)$ equals

$$f'(x) = g'(x) \cdot h(x) + g(x) \cdot h'(x)$$

The derivative of $f(x) = g(x) \cdot h(x)$, with $g(x) = x^2$ and $h(x) = \sin(x)$ equals

$$\begin{aligned} f'(x) &= g'(x) \cdot h(x) + g(x) \cdot h'(x) \\ &= 2x \cdot \sin(x) + \end{aligned}$$

The derivative of $f(x) = g(x) \cdot h(x)$, with $g(x) = x^2$ and $h(x) = \sin(x)$ equals

$$\begin{aligned} f'(x) &= g'(x) \cdot h(x) + g(x) \cdot h'(x) \\ &= 2x \cdot \sin(x) + x^2 \cdot \cos(x). \end{aligned}$$